some basic operations generlized

arch/otbn/abstraction.i.dfy
@@ -1,8 +1,90 @@
 include "machine.s.dfy"
 
 module ot_abstraction {
-    import opened bv_ops
+    import opened integers
+    import opened bv256_ops
     import opened ot_machine
+
+/* safe stateless operations */
+
+    // quater shift but no overflow
+
+    predicate otbn_qshift_is_safe(x: uint256, q: uint2)
+    {
+        && (q == 1 ==> x < BASE_192)
+        && (q == 2 ==> x < BASE_128)
+        && (q == 3 ==> x < BASE_64)
+    }
+
+    function otbn_qshift_safe(x: uint256, q: uint2): (r: uint256)
+        requires otbn_qshift_is_safe(x, q);
+    {
+        if q == 0 then x
+        else if q == 1 then x * BASE_64
+        else if q == 2 then x * BASE_128
+        else x * BASE_192
+    }
+
+    lemma otbn_qshift_safe_correct_lemma(x: uint256, q: uint2)
+        requires otbn_qshift_is_safe(x, q);
+        ensures otbn_qshift_safe(x, q) == otbn_shift(x, SFT(true, q * 8));
+    {
+        var num_bytes := q * 8;
+        assert 0 <= num_bytes <= 24;
+        var shift := SFT(true, num_bytes);
+        var num_bits := num_bytes * 8;
+        var result := bv256_ops.ls(x, num_bits);
+        ls_is_mul(x, num_bytes, result);
+        assert otbn_qshift_safe(x, q) == otbn_shift(x, shift);
+    }
+
+    // predicate otbn_mulqacc_is_safe(acc: uint256, shift: uint2, x:)
+    // {
+    //     // make sure no overflow from shift (product needs to be 128 bits)
+    //     && (shift <= 2) 
+    //     // make sure no overflow from addtion
+    //     && (acc + otbn_qshift_safe(x, shift) < BASE_256)
+    // }
+
+    // // mulqacc but no overflow
+    // function otbn_mulqacc_safe(
+    //     zero: bool,
+    //     x: uint256, qx: uint2,
+    //     y: uint256, qy: uint2,
+    //     shift: uint2,
+    //     acc: uint256) : uint256
+
+    //     requires otbn_mulqacc_is_safe(shift, acc);
+    // {
+    //     var product := otbn_qmul(x, qx, y, qy);
+    //     var shift := otbn_qshift_safe(product, shift * 8);
+    //     if zero then shift else acc + shift
+    // }
+
+    // lemma otbn_mulqacc_safe_correct_lemma(
+    //     zero: bool,
+    //     x: uint256, qx: uint2,
+    //     y: uint256, qy: uint2,
+    //     shift: uint2,
+    //     acc: uint256)
+    //     requires otbn_mulqacc_is_safe(shift, acc);
+    //     ensures otbn_mulqacc_safe(zero, x, qx, y, qy, shift, acc)
+    //         == otbn_mulqacc(zero, x, qx, y, qy, shift, acc);
+    // {
+    //     // var result1 := otbn_mulqacc_safe(zero, x, qx, y, qy, shift, acc);
+    //     // // var result2 := otbn_mulqacc(zero, x, qx, y, qy, shift, acc);
+
+    //     // var product := otbn_qmul(x, qx, y, qy);
+    //     // var shifted1 := otbn_qshift_safe(product, shift);
+    //     // assert result1 == if zero then shifted1 else acc + shifted1;
+
+    //     // otbn_qshift_safe_correct_lemma(x, shift);
+
+    //     // var shifted2 := otbn_qshift_safe(product, shift);
+    //     // assert result2 == if zero then shift else bv256_ops.add(acc, shift);
+
+    //     assume false;
+    // }
 
 /* wdr_view definion (SHADOW) */
 
@@ -259,7 +341,7 @@ module ot_abstraction {
             {
                 assert wword_inv(heap, mem, base_ptr, i, buff[i]);
                 if i == j {
-                    uint256_eighth_value(value);
+                    eighth_value(value);
                     assert wword_inv(heap', mem', base_ptr, i, value);
                 }
             }
@@ -356,6 +438,108 @@ module ot_abstraction {
             ensures heap_xword_inv(heap', mem', base_ptr)
         {
             assert heap_xword_inv(heap, mem, base_ptr);
+        }
+    }
+
+/* debug prints */
+
+    method print_as_hex(a: nat, bytes: nat)
+    {
+        var val := a;
+        var num_digits := bytes * 2;
+        var i := 0;
+        var result := "";
+        while i < num_digits
+            decreases num_digits - i
+        {
+            var digit := val % 16;
+            if digit == 0 {
+                result := "0" + result;
+            } else if digit == 1 {
+                result := "1" + result;
+            } else if digit == 2 {
+                result := "2" + result;
+            } else if digit == 3 {
+                result := "3" + result;
+            } else if digit == 4 {
+                result := "4" + result;
+            } else if digit == 5 {
+                result := "5" + result;
+            } else if digit == 6 {
+                result := "6" + result;
+            } else if digit == 7 {
+                result := "7" + result;
+            } else if digit == 8 {
+                result := "8" + result;
+            } else if digit == 9 {
+                result := "9" + result;
+            } else if digit == 10 {
+                result := "a" + result;
+            } else if digit == 11 {
+                result := "b" + result;
+            } else if digit == 12 {
+                result := "c" + result;
+            } else if digit == 13 {
+                result := "d" + result;
+            } else if digit == 14 {
+                result := "e" + result;
+            } else if digit == 15 {
+                result := "f" + result;
+            }
+            val := val / 16;
+            i := i + 1;
+        }
+        print("0x"); print(result);
+    }
+
+    method dump_regs(s: state)
+    {
+        var i := 0;
+        while i < 32
+        {
+            print(" x"); print(i); 
+            if i < 10 {
+                print("  = ");
+            } else {
+                print(" = ");
+            }
+            print_as_hex(s.read_reg32(GPR(i)), 4); print("\n"); 
+            i := i + 1;
+        }
+
+        i := 0;
+        while i < 32
+        {
+            print(" w"); print(i);
+            if i < 10 {
+                print("  = ");
+            } else {
+                print(" = ");
+            }
+            print_as_hex(s.read_reg256(WDR(i)), 32); print("\n"); 
+            i := i + 1;
+        }
+
+        print(" fg0 = ");print_as_hex(s.fgroups.fg0.to_nat(), 4); print("\n"); 
+        print(" fg1 = ");print_as_hex(s.fgroups.fg1.to_nat(), 4); print("\n"); 
+    }
+
+    method dump_mem(s: state, addr: uint32, words: uint32)
+        requires xword_ptr_admissible(addr + words * 4)
+    {
+        var end := addr + words * 4;
+        var cur := addr;
+        var i := 0;
+
+        while cur < end
+            invariant cur == addr + i * 4
+            invariant xword_ptr_admissible(cur)
+            decreases end - cur
+        {
+            var value := s.read_xword(cur);
+            print(cur); print(":"); print_as_hex(value, 4); print("\n");
+            cur := cur + 4;
+            i := i + 1;
         }
     }
 }
