impl/dafny/generic_bv_ops.dfy
@@ -1,0 +1,64 @@
+include "../../std_lib/src/Collections/Sequences/LittleEndianNat.dfy"
+
+abstract module generic_bv_ops
+{
+    import opened BVSEQ: LittleEndianNat
+    import Mul
+
+    type uint1   = i :int | 0 <= i < 2
+    
+    // half word base
+    function method HW_BASE(): nat
+        ensures HW_BASE() > 1
+        ensures HW_BASE() * HW_BASE() == BASE()
+
+    // double word base
+    function method DW_BASE(): nat
+    {
+        Mul.LemmaMulStrictlyPositiveAuto();
+        BASE() * BASE()
+    }
+
+    function method bool_to_uint1(i:bool) : uint1
+    {
+        if i then 1 else 0
+    }
+
+    function method uint_addc(x: uint, y: uint, cin: uint1): (uint, uint1)
+    {
+        var sum : int := x + y + cin;
+        var sum_out := if sum < BASE() then sum else sum - BASE();
+        var cout := if sum  < BASE() then 0 else 1;
+        (sum_out, cout)
+    }
+
+    function method uint_add(x: uint, y: uint): uint
+    {
+        uint_addc(x, y, 0).0
+    }
+
+    function method uint_subb(x: uint, y: uint, bin: uint1): (uint, uint1)
+    {
+        var diff : int := x - y - bin;
+        var diff_out := if diff >= 0 then diff else diff + BASE();
+        var bout := if diff >= 0 then 0 else 1;
+        (diff_out, bout)
+    }
+
+    function method uint_sub(x: uint, y: uint) : uint
+    {
+        uint_subb(x, y, 0).0
+    }
+
+    function method uint_and(x: uint, y: uint): uint
+
+    function method uint_or(x: uint, y: uint): uint
+
+    function method uint_not(x: uint) : uint
+
+    function method uint_xor(x: uint, y: uint): uint
+
+    function method uint_rs(x: uint, amount: uint): uint
+
+    function method uint_ls(x: uint, amount: uint): uint
+} 
