impl/dafny/generic_dw_add_lemmas.i.dfy
@@ -1,0 +1,189 @@
+include "generic_bv_ops.dfy"
+
+abstract module generic_dw_add_lemmas {
+    import opened GBV: generic_bv_ops
+    import opened GBV.BVSEQ
+    import opened Mul
+    import opened Power
+    import opened DivMod
+
+    predicate uint_dw_add_is_safe(
+        x_lh: uint, x_uh: uint,
+        y_lh: uint, y_uh: uint)
+    {
+        ToNatRight([x_lh, x_uh]) + ToNatRight([y_lh, y_uh]) < DW_BASE()
+    }
+
+    lemma uint_dw_add_lemma(
+        x_lh: uint, x_uh: uint,
+        y_lh: uint, y_uh: uint,
+        c1: uint1, c2: uint1,
+        z_lh: uint, z_uh: uint)
+
+        requires uint_dw_add_is_safe(x_lh, x_uh, y_lh, y_uh);
+        requires (z_lh, c1) == uint_addc(x_lh, y_lh, 0);
+        requires (z_uh, c2) == uint_addc(x_uh, y_uh, c1);
+        
+        ensures ToNatRight([z_lh, z_uh]) == ToNatRight([x_lh, x_uh]) + ToNatRight([y_lh, y_uh]);
+    {
+        var x_full := ToNatRight([x_lh, x_uh]);
+        var y_full := ToNatRight([y_lh, y_uh]);
+        var z_full := ToNatRight([z_lh, z_uh]);
+
+        assert SeqAdd([x_lh], [y_lh]) == ([z_lh], c1) by {
+            reveal SeqAdd();
+            assert [] + [z_lh] == [z_lh];
+        }
+
+        assert SeqAdd([x_lh, x_uh], [y_lh, y_uh]) == ([z_lh, z_uh], c2) by {
+            reveal SeqAdd();
+            assert [z_lh] + [z_uh] == [z_lh, z_uh];
+        }
+
+        assert ToNatRight([z_lh, z_uh]) + c2 * Pow(BASE(), 2) == x_full + ToNatRight([y_lh, y_uh]) by {
+            LemmaSeqAdd([x_lh, x_uh], [y_lh, y_uh], [z_lh, z_uh], c2);
+        }
+
+        if c2 != 0 {
+            reveal Pow();
+            assert false;
+        }
+    }
+
+    method dw_add(x_lh: uint, x_uh: uint, y_lh: uint, y_uh: uint)
+        requires uint_dw_add_is_safe(x_lh, x_uh, y_lh, y_uh);
+    {
+        var (z_lh, c1) := uint_addc(x_lh, y_lh, 0);
+        var (z_uh, c2) := uint_addc(x_uh, y_uh, c1);
+        uint_dw_add_lemma(x_lh, x_uh, y_lh, y_uh, c1, c2, z_lh, z_uh);
+    }
+
+    method full_mul(a: uint, b: uint) returns (lh: uint, uh: uint)
+        ensures a * b == ToNatRight([lh, uh])
+    {
+        var full := a * b;
+
+        assert full >= 0 by {
+            LemmaMulNonnegativeAuto();
+        }
+
+        assert full < BASE() * BASE() by {
+            full_mul_bound_lemma(a, b);
+        }
+
+        ghost var glh := full % BASE();
+        ghost var guh := full / BASE();
+
+        assert BASE() * guh + glh == full by {
+            LemmaFundamentalDivModAuto();
+        }
+
+        if guh >= BASE() {
+            assert full >= BASE() * BASE() + glh by {
+                LemmaMulIsCommutativeAuto();
+                LemmaMulInequalityAuto();
+            }
+            assert false;
+        }
+
+        assert guh >= 0 by {
+            LemmaDivPosIsPos(full, BASE());
+        }
+
+        lh := full % BASE();
+        uh := full / BASE();
+
+        assert a * b == ToNatRight([lh, uh]) by {
+            LemmaMulIsCommutativeAuto();
+            LemmaSeqLen2([lh, uh]);
+        }
+    }
+
+    lemma full_mul_bound_lemma(a: uint, b: uint)
+        ensures a * b < DW_BASE();
+        ensures a * b <= (BASE() - 1) * (BASE() - 1)
+    {
+        var full := a * b;
+
+        assert full <= (BASE() - 1) * (BASE() - 1) by {
+            LemmaMulUpperBoundAuto();
+        }
+
+        assert full < BASE() * BASE() by {
+            calc <= {
+                full;
+                (BASE() - 1) * (BASE() - 1);
+                {
+                    LemmaMulIsDistributiveSubAuto();
+                }
+                (BASE() - 1) * BASE() - (BASE() - 1);
+                {
+                    LemmaMulIsCommutativeAuto();
+                    LemmaMulIsDistributiveSubAuto();
+                }
+                BASE() * BASE() - BASE() - (BASE() - 1);
+                BASE() * BASE() - 2 * BASE() + 1;
+            }
+        }
+    }
+
+    lemma mul_add_bound_lemma(a: uint, b: uint, c: uint)
+       ensures a * b + c < DW_BASE();
+    {
+        var u := BASE() - 1;
+        calc {
+            a * b + c;
+            <= { full_mul_bound_lemma(a, b); }
+            u * u + c;
+            <=
+            u * u + u;
+            == { LemmaMulIsDistributiveAddAuto(); }
+            u * (u + 1); 
+            <  { LemmaMulLeftInequality(u + 1, u, u + 1); }
+            (u + 1) * (u + 1); 
+            ==
+            DW_BASE();
+        }
+    }
+    
+    method mul_add(a: uint, b: uint, c: uint) returns (lh: uint, uh: uint)
+    {
+        var p_lh, p_uh := full_mul(a, b);
+
+        var res1 := uint_addc(p_lh, c, 0);
+        var res2 := uint_addc(p_uh, 0, res1.1);
+        lh, uh := res1.0, res2.0;
+
+        mul_add_bound_lemma(a, b, c);
+
+        assert ToNatRight([c, 0]) == c by {
+            LemmaSeqLen2([c, 0]);
+            assert ToNatRight([c, 0]) == c + 0 * BASE();
+        }
+        uint_dw_add_lemma(p_lh, p_uh, c, 0, res1.1, res2.1, lh, uh);
+    }
+
+    lemma mul_double_add_bound_lemma(a: uint, b: uint, c: uint, d: uint)
+        ensures a * b + c + d < DW_BASE();
+    {
+        var u := BASE() - 1;
+
+        calc {
+            a * b + c + d;
+            <= { full_mul_bound_lemma(a, b); }
+            u * u + c + d;
+            <= u * u + u + u;
+            u * u + 2 * u;
+            < (u * u) + (2 * u) + 1;
+        }
+
+        calc == {
+            (u + 1) * (u + 1);
+            { LemmaMulIsDistributiveAdd(u + 1, u, 1); }
+            (u + 1) * u + (u + 1) * 1; 
+            u * (u + 1) + u + 1;
+            { LemmaMulIsDistributiveAdd(u, u, 1); }
+            (u * u) + (2 * u) + 1;
+        }
+    }
+}
