lib/bv32_ops.dfy
@@ -1,0 +1,57 @@
+include "generic_bv_ops.dfy"
+
+module bv32_seq refines LittleEndianNat
+{
+    import integers
+
+    function method BASE(): nat
+    {
+        integers.BASE_32
+    }
+}
+
+module bv32_ops refines generic_bv_ops
+{
+    import opened BVSEQ = bv32_seq 
+
+    // half word base
+    function method HW_BASE(): nat
+    {
+        integers.BASE_16
+    }
+
+    function method {:opaque} and(x: uint, y: uint): uint
+    {
+        (x as bv32 & y as bv32) as uint
+    }
+
+    function method {:opaque} or(x: uint, y: uint): uint
+    {
+       (x as bv32 | y as bv32) as uint
+    }
+
+    function method {:opaque} not(x: uint) : uint
+    {
+        !(x as bv32) as uint
+    }
+
+    function method {:opaque} xor(x: uint, y: uint): uint
+    {
+       (x as bv32 ^ y as bv32) as uint
+    }
+
+    predicate valid_shift(amount: uint)
+    {
+        amount <= 32
+    }
+
+    function method {:opaque} rs(x: uint, amount: uint): uint
+    {
+        (x as bv32 >> amount) as uint
+    }
+
+    function method {:opaque} ls(x: uint, amount: uint): uint
+    {
+        (x as bv32 << amount) as uint
+    }
+} 
