lib/generic_bv_ops.dfy
@@ -1,0 +1,242 @@
+include "../std_lib/src/Collections/Sequences/LittleEndianNat.dfy"
+include "../std_lib/src/BoundedInts.dfy"
+
+module integers
+{
+    import BoundedInts
+
+    const BASE_1   : int := BoundedInts.TWO_TO_THE_1
+    const BASE_2   : int := BoundedInts.TWO_TO_THE_2
+    const BASE_4   : int := BoundedInts.TWO_TO_THE_4
+    const BASE_5   : int := BoundedInts.TWO_TO_THE_5
+    const BASE_8   : int := BoundedInts.TWO_TO_THE_8
+    const BASE_16  : int := BoundedInts.TWO_TO_THE_16
+    const BASE_32  : int := BoundedInts.TWO_TO_THE_32
+    const BASE_64  : int := BoundedInts.TWO_TO_THE_64
+    const BASE_128 : int := BoundedInts.TWO_TO_THE_128
+    const BASE_192 : int := 0x1_00000000_00000000_00000000_00000000_00000000_00000000
+    const BASE_256 : int := BoundedInts.TWO_TO_THE_256
+    const BASE_512 : int := BoundedInts.TWO_TO_THE_512
+
+    type uint1   = i :int | 0 <= i < BASE_1
+    type uint2   = i :int | 0 <= i < BASE_2
+    type uint4   = i :int | 0 <= i < BASE_4
+    type uint5   = i :int | 0 <= i < BASE_5
+    type uint10  = i :int | 0 <= i < 1024
+    type uint32  = i :int | 0 <= i < BASE_32
+    type uint64  = i :int | 0 <= i < BASE_64
+    type uint128 = i :int | 0 <= i < BASE_128
+    type uint192 = i :int | 0 <= i < BASE_192
+    type uint256 = i :int | 0 <= i < BASE_256
+    type uint512 = i :int | 0 <= i < BASE_512
+
+    type int10   = i :int | -512 <= i <= 511
+    type int12   = i :int | -2048 <= i <= 2047
+}
+
+abstract module generic_bv_ops
+{
+    import opened BVSEQ: LittleEndianNat
+    import Mul
+    import DivMod
+
+    import integers
+
+    type uint1 = integers.uint1
+
+    // the singed version of uint
+    type sint = i: int | -(BASE() as int) < i < BASE() as int
+
+    // half word base
+    function method HW_BASE(): nat
+        ensures 1 < HW_BASE() < BASE()
+        ensures HW_BASE() * HW_BASE() == BASE()
+
+    // double word base
+    function method DW_BASE(): nat
+    {
+        Mul.LemmaMulStrictlyPositiveAuto();
+        BASE() * BASE()
+    }
+
+    function method bool_to_uint1(i:bool): uint1
+    {
+        if i then 1 else 0
+    }
+
+    function method and(x: uint, y: uint): uint
+
+    function method or(x: uint, y: uint): uint
+
+    function method not(x: uint) : uint
+
+    function method xor(x: uint, y: uint): uint
+
+    predicate valid_shift(amount: uint)
+
+    function method rs(x: uint, amount: uint): uint
+        requires valid_shift(amount)
+
+    function method ls(x: uint, amount: uint): uint
+        requires valid_shift(amount)
+
+    function method {:opaque} lsb(x: uint): uint1
+    {
+        x % 2
+    }
+
+    function method msb(x: uint): uint1
+
+/* addition */
+
+    function method addc(x: uint, y: uint, cin: uint1): (uint, uint1)
+    {
+        var sum : int := x + y + cin;
+        var sum_out := if sum < BASE() then sum else sum - BASE();
+        var cout := if sum  < BASE() then 0 else 1;
+        (sum_out, cout)
+    }
+
+    function method add(x: uint, y: uint): uint
+    {
+        addc(x, y, 0).0
+    }
+
+    function method to_2s_comp(n: sint): uint
+    {
+        if n < 0 then n + BASE() else n
+    }
+
+    function method addi(x: uint, imm: sint): uint
+    {
+        add(x, to_2s_comp(imm))
+    }
+
+/* subtraction */
+
+    function method subb(x: uint, y: uint, bin: uint1): (uint, uint1)
+    {
+        var diff : int := x - y - bin;
+        var diff_out := if diff >= 0 then diff else diff + BASE();
+        var bout := if diff >= 0 then 0 else 1;
+        (diff_out, bout)
+    }
+
+    function method sub(x: uint, y: uint): uint
+    {
+        subb(x, y, 0).0
+    }
+
+/* upper/lower half split */
+
+    function method {:opaque} lh(x: uint): uint
+        ensures lh(x) < HW_BASE()
+    {
+        x % HW_BASE()
+    }
+
+    lemma upper_half_bound_lemma(x: uint)
+        ensures 0 <= x / HW_BASE() < HW_BASE()
+    {
+        var d := HW_BASE();
+        var lh, uh := x % d, x / d;
+
+        DivMod.LemmaFundamentalDivMod(x, d);
+
+        assert x == lh + uh * d;
+
+        if uh > HW_BASE() {
+            Mul.LemmaMulIsCommutativeAuto();
+            Mul.LemmaMulInequalityAuto();
+            assert false;
+        }
+        DivMod.LemmaDivPosIsPos(x, d);
+    }
+
+    function method {:opaque} uh(x: uint): uint
+        ensures uh(x) < HW_BASE()
+    {
+        upper_half_bound_lemma(x);
+        x / HW_BASE()
+    }
+
+    lemma half_split_lemma(x: uint)
+        ensures x == lh(x) + uh(x) * HW_BASE();
+    {
+        DivMod.LemmaFundamentalDivMod(x, HW_BASE());
+        Mul.LemmaMulIsCommutativeAuto();
+        reveal lh();
+        reveal uh();
+    }
+
+/* mul_add bounds */
+
+    lemma full_mul_bound_lemma(a: uint, b: uint)
+        ensures a * b < DW_BASE();
+        ensures a * b <= (BASE() - 1) * (BASE() - 1)
+    {
+        var full := a * b;
+
+        assert full <= (BASE() - 1) * (BASE() - 1) by {
+            Mul.LemmaMulUpperBoundAuto();
+        }
+
+        assert full < BASE() * BASE() by {
+            calc <= {
+                full;
+                (BASE() - 1) * (BASE() - 1);
+                { Mul.LemmaMulIsDistributiveSubAuto(); }
+                (BASE() - 1) * BASE() - (BASE() - 1);
+                {
+                    Mul.LemmaMulIsCommutativeAuto();
+                    Mul.LemmaMulIsDistributiveSubAuto();
+                }
+                BASE() * BASE() - BASE() - (BASE() - 1);
+                BASE() * BASE() - 2 * BASE() + 1;
+            }
+        }
+    }
+
+    lemma mul_add_bound_lemma(a: uint, b: uint, c: uint)
+       ensures a * b + c < DW_BASE();
+    {
+        var u := BASE() - 1;
+        calc {
+            a * b + c;
+            <= { full_mul_bound_lemma(a, b); }
+            u * u + c;
+            <=
+            u * u + u;
+            == { Mul.LemmaMulIsDistributiveAddAuto(); }
+            u * (u + 1); 
+            <  { Mul.LemmaMulLeftInequality(u + 1, u, u + 1); }
+            (u + 1) * (u + 1); 
+            ==
+            DW_BASE();
+        }
+    }
+    
+    lemma mul_double_add_bound_lemma(a: uint, b: uint, c: uint, d: uint)
+        ensures a * b + c + d < DW_BASE();
+    {
+        var u := BASE() - 1;
+
+        calc {
+            a * b + c + d;
+            <= { full_mul_bound_lemma(a, b); }
+            u * u + c + d;
+            <= u * u + u + u;
+            u * u + 2 * u;
+            < (u * u) + (2 * u) + 1;
+        }
+
+        calc == {
+            (u + 1) * (u + 1);
+            { Mul.LemmaMulIsDistributiveAdd(u + 1, u, 1); }
+            (u + 1) * u + (u + 1) * 1; 
+            u * (u + 1) + u + 1;
+            { Mul.LemmaMulIsDistributiveAdd(u, u, 1); }
+            (u * u) + (2 * u) + 1;
+        }
+    }
+}
